Delete old files

src/tactic/vampire/list.lean
@@ -1,136 +1,11 @@
-/-
-  Copyright (c) 2019 Seul Baek. All rights reserved.
-  Released under Apache 2.0 license as described in the file LICENSE.
-  Author: Seul Baek
-
-  List lemmas and definitions.
--/
-
 import data.list.basic
 import tactic.vampire.misc
 
-universes u v
-
-variables {α : Type u} {β : Type v}
-
 namespace list
 
-def remove_one [decidable_eq α] (a : α) (as : list α) : option (list α) :=
-if as.index_of a < as.length
-then some (as.remove_nth $ as.index_of a)
-else none
+variables {α β : Type}
 
-lemma exists_mem_iff_exists_mem_map
-  {p : α → Prop} {q : β → Prop} {f : α → β} (h : ∀ a : α, q (f a) ↔ p a) :
-  ∀ as : list α, ((∃ b ∈ as.map f, q b) ↔ (∃ a ∈ as, p a))
-| []        := by constructor; rintro ⟨_, ⟨_⟩, _⟩
-| (a :: as) :=
-  begin
-    rw [map_cons],
-    simp only [exists_mem_cons_iff],
-    apply pred_mono_2 (h _),
-    apply exists_mem_iff_exists_mem_map
-  end
-
-def exteq [decidable_eq α] : list α → list α → Prop
-| []        []       := true
-| []        (_ :: _) := false
-| (a :: l1) l2       :=
-  match l2.remove_one a with
-  | none       := false
-  | (some l2') := exteq l1 l2'
-  end
-
-lemma mem_remove_nth {a : α}  :
-  ∀ l : list α, ∀ k m : nat,
-  l.nth m = some a → k ≠ m → a ∈ l.remove_nth k
-| [] k m h0 h1 := by cases h0
-| (b :: l) 0 m h0 h1 :=
-  begin
-    cases m, {cases h1 rfl},
-    simp only [list.remove_nth],
-    rw list.mem_iff_nth, use m,
-    exact h0
-  end
-| (b :: l) (k + 1) m h0 h1 :=
-  begin
-    cases m,
-    { apply or.inl (option.some.inj h0.symm) },
-    have h2 : k ≠ m,
-    { intro h2, rw h2 at h1, cases h1 rfl },
-    apply or.inr (mem_remove_nth _ k m h0 h2)
-  end
-
-lemma mem_of_mem_remove_nth {a : α} :
-  ∀ l : list α, ∀ k : nat, a ∈ l.remove_nth k → a ∈ l
-| []       k h0 := by cases k; cases h0
-| (b :: l) 0 h0 := or.inr h0
-| (b :: l) (k + 1) h0 :=
-  by { cases h0, {exact or.inl h0},
-       apply or.inr (mem_of_mem_remove_nth l k h0) }
-
-lemma mem_iff_nth_eq_some_or_mem_remove_nth
-  {a : α} {l : list α} (k : nat) :
-  a ∈ l ↔ (a ∈ l.remove_nth k ∨ l.nth k = some a) :=
-begin
-  constructor; intro h0,
-  { rw @list.mem_iff_nth _ a l at h0,
-    rcases h0 with ⟨m, h1⟩,
-    by_cases h2 : k = m,
-    { right, rwa ← h2 at h1 },
-    left, apply mem_remove_nth _ _ _ h1 h2 },
-  cases h0,
-  { apply mem_of_mem_remove_nth _ _ h0 },
-  rw @list.mem_iff_nth _ a l,
-  refine ⟨k, h0⟩
-end
-
-lemma remove_one_subset [decidable_eq α] (a : α) (l1 l2 : list α) :
-  l1.remove_one a = some l2 → l2 ⊆ l1 :=
-begin
-  unfold list.remove_one,
-  by_cases l1.index_of a < l1.length,
-  { rw if_pos h, intro h1,
-    rw ← (option.some.inj h1),
-    intros x h2,
-    rw list.mem_iff_nth_eq_some_or_mem_remove_nth (l1.index_of a),
-    left, assumption },
-  rw if_neg h, rintro ⟨_⟩
-end
-
-lemma subset_of_exteq [decidable_eq α] :
-  ∀ l1 l2 : list α, list.exteq l1 l2 → l1 ⊆ l2
-| []        []       h0 x h1 := by cases h1
-| []        (_ :: _) h0 x h1 := by cases h0
-| (a :: l1) l2       h0 x h1 :=
-  begin
-    unfold list.exteq at h0,
-    cases h2 : (l2.remove_one a) with l2',
-    { rw h2 at h0, cases h0 },
-    cases h1,
-    { subst h1,
-      unfold list.remove_one at h2,
-      by_cases h3 : l2.index_of x < l2.length,
-      { rw list.index_of_lt_length at h3, exact h3 },
-      rw if_neg h3 at h2, cases h2 },
-    rw h2 at h0,
-    have h3 := subset_of_exteq _ _ h0,
-    apply list.remove_one_subset _ _ _ h2 (h3 h1)
-  end
-
-instance decidable_exteq [decidable_eq α] :
-  ∀ l1 l2 : list α, decidable (list.exteq l1 l2)
-| []        []       := by { right, trivial }
-| []        (_ :: _) := by { left, rintro ⟨_⟩ }
-| (a :: l1) l2       :=
-  begin
-    unfold list.exteq,
-    cases (l2.remove_one a),
-    { left, rintro ⟨_⟩ },
-    apply decidable_exteq,
-  end
-
-theorem exists_mem_append {p : α → Prop} {l₁ l₂ : list α} :
+lemma exists_mem_append {p : α → Prop} {l₁ l₂ : list α} :
   (∃ x ∈ l₁ ++ l₂, p x) ↔ (∃ x ∈ l₁, p x) ∨ (∃ x ∈ l₂, p x) :=
 begin
   constructor; intro h0,
@@ -147,19 +22,19 @@ def rot : nat → list α → list α
 | _ [] := []
 | 0 (a :: as) := (a :: as)
 | (k + 1) (a :: as) :=
-  match (as.rot k) with
+  match (rot k as) with
   | [] := (a :: as)
   | (a' :: as') := (a' :: a :: as')
   end
 
 lemma mem_rot {a : α} :
-  ∀ {as : list α}, ∀ k : nat, a ∈ as → a ∈ as.rot k
+  ∀ {as : list α}, ∀ k : nat, a ∈ as → a ∈ rot k as
 | [] _ h0 := by cases h0
 | (b :: as) 0 h0 := h0
 | (b :: as) (k + 1) h0 :=
   begin
     cases h0; unfold rot;
-    cases h1 : (as.rot k) with b' as',
+    cases h1 : (rot k as) with b' as',
     { left, assumption },
     { right, left, assumption },
     { right, assumption },
@@ -169,176 +44,18 @@ lemma mem_rot {a : α} :
     right, right, assumption
   end
 
-  #exit
-
-lemma exists_mem_iff_exists_mem_map
-  {p : α → Prop} {q : β → Prop} {f : α → β} (h : ∀ a : α, p a ↔ q (f a)) :
-  ∀ as : list α, ((∃ a ∈ as, p a) ↔ (∃ b ∈ as.map f, q b))
+lemma exists_mem_map_iff
+  {p : α → Prop} {q : β → Prop} {f : α → β}
+  (h : ∀ a : α, q (f a) ↔ p a) :
+  ∀ as : list α,
+  ((∃ b ∈ as.map f, q b) ↔ (∃ a ∈ as, p a))
 | []        := by constructor; rintro ⟨_, ⟨_⟩, _⟩
 | (a :: as) :=
   begin
-    rw [map_cons],
-    simp only [exists_mem_cons_iff],
+    rw [list.map_cons],
+    simp only [list.exists_mem_cons_iff],
     apply pred_mono_2 (h _),
-    apply exists_mem_iff_exists_mem_map
-  end
-
-lemma forall_mem_iff_forall_mem_map
-  {p : α → Prop} {q : β → Prop} {f : α → β} (h : ∀ a : α, p a ↔ q (f a)) :
-  ∀ as : list α, ((∀ a ∈ as, p a) ↔ (∀ b ∈ as.map f, q b))
-| []        := by constructor; intro; apply forall_mem_nil
-| (a :: as) :=
-  begin
-    rw [map_cons],
-    simp only [forall_mem_cons],
-    apply pred_mono_2 (h _),
-    apply forall_mem_iff_forall_mem_map
-  end
-
-
-def halve (l : list α) : list α × list α :=
-split_at (l.length / 2) l
-
-end list
-
-
-#exit
-universes u v
-
-variables {α : Type u} {β : Type v}
-
-namespace list
-
-open option
-
-lemma exists_mem_iff_exists_mem_map
-  {p : α → Prop} {q : β → Prop} {f : α → β} (h : ∀ a : α, p a ↔ q (f a)) :
-  ∀ as : list α, ((∃ a ∈ as, p a) ↔ (∃ b ∈ as.map f, q b))
-| []        := by constructor; rintro ⟨_, ⟨_⟩, _⟩
-| (a :: as) :=
-  begin
-    rw [map_cons],
-    simp only [exists_mem_cons_iff],
-    apply pred_mono_2 (h _),
-    apply exists_mem_iff_exists_mem_map
-  end
-
-lemma forall_mem_iff_forall_mem_map
-  {p : α → Prop} {q : β → Prop} {f : α → β} (h : ∀ a : α, p a ↔ q (f a)) :
-  ∀ as : list α, ((∀ a ∈ as, p a) ↔ (∀ b ∈ as.map f, q b))
-| []        := by constructor; intro; apply forall_mem_nil
-| (a :: as) :=
-  begin
-    rw [map_cons],
-    simp only [forall_mem_cons],
-    apply pred_mono_2 (h _),
-    apply forall_mem_iff_forall_mem_map
-  end
-
-
-lemma mem_remove_nth {a : α}  :
-  ∀ l : list α, ∀ k m : nat,
-  l.nth m = some a → k ≠ m → a ∈ l.remove_nth k
-| [] k m h0 h1 := by cases h0
-| (b :: l) 0 m h0 h1 :=
-  begin
-    cases m, {cases h1 rfl},
-    simp only [list.remove_nth],
-    rw list.mem_iff_nth, use m,
-    exact h0
-  end
-| (b :: l) (k + 1) m h0 h1 :=
-  begin
-    cases m,
-    { apply or.inl (option.some.inj h0.symm) },
-    have h2 : k ≠ m,
-    { intro h2, rw h2 at h1, cases h1 rfl },
-    apply or.inr (mem_remove_nth _ k m h0 h2)
-  end
-
-lemma mem_of_mem_remove_nth {a : α} :
-  ∀ l : list α, ∀ k : nat, a ∈ l.remove_nth k → a ∈ l
-| []       k h0 := by cases k; cases h0
-| (b :: l) 0 h0 := or.inr h0
-| (b :: l) (k + 1) h0 :=
-  by { cases h0, {exact or.inl h0},
-       apply or.inr (mem_of_mem_remove_nth l k h0) }
-
-lemma mem_iff_nth_eq_some_or_mem_remove_nth
-  {a : α} {l : list α} (k : nat) :
-  a ∈ l ↔ (a ∈ l.remove_nth k ∨ l.nth k = some a) :=
-begin
-  constructor; intro h0,
-  { rw @list.mem_iff_nth _ a l at h0,
-    rcases h0 with ⟨m, h1⟩,
-    by_cases h2 : k = m,
-    { right, rwa ← h2 at h1 },
-    left, apply mem_remove_nth _ _ _ h1 h2 },
-  cases h0,
-  { apply mem_of_mem_remove_nth _ _ h0 },
-  rw @list.mem_iff_nth _ a l,
-  refine ⟨k, h0⟩
-end
-
-def remove_one [decidable_eq α] (a : α) (as : list α) : option (list α) :=
-if as.index_of a < as.length
-then some (as.remove_nth $ as.index_of a)
-else none
-
-/- Equivalent to perm, but includes no axioms -/
-
-def exteq [decidable_eq α] : list α → list α → Prop
-| []        []       := true
-| []        (_ :: _) := false
-| (a :: l1) l2       :=
-  match l2.remove_one a with
-  | none       := false
-  | (some l2') := exteq l1 l2'
-  end
-
-lemma remove_one_subset [decidable_eq α] (a : α) (l1 l2 : list α) :
-  l1.remove_one a = some l2 → l2 ⊆ l1 :=
-begin
-  unfold list.remove_one,
-  by_cases l1.index_of a < l1.length,
-  { rw if_pos h, intro h1,
-    rw ← (option.some.inj h1),
-    intros x h2,
-    rw list.mem_iff_nth_eq_some_or_mem_remove_nth (l1.index_of a),
-    left, assumption },
-  rw if_neg h, rintro ⟨_⟩
-end
-
-lemma subset_of_exteq [decidable_eq α] :
-  ∀ l1 l2 : list α, list.exteq l1 l2 → l1 ⊆ l2
-| []        []       h0 x h1 := by cases h1
-| []        (_ :: _) h0 x h1 := by cases h0
-| (a :: l1) l2       h0 x h1 :=
-  begin
-    unfold list.exteq at h0,
-    cases h2 : (l2.remove_one a) with l2',
-    { rw h2 at h0, cases h0 },
-    cases h1,
-    { subst h1,
-      unfold list.remove_one at h2,
-      by_cases h3 : l2.index_of x < l2.length,
-      { rw list.index_of_lt_length at h3, exact h3 },
-      rw if_neg h3 at h2, cases h2 },
-    rw h2 at h0,
-    have h3 := subset_of_exteq _ _ h0,
-    apply list.remove_one_subset _ _ _ h2 (h3 h1)
-  end
-
-instance decidable_exteq [decidable_eq α] :
-  ∀ l1 l2 : list α, decidable (list.exteq l1 l2)
-| []        []       := by { right, trivial }
-| []        (_ :: _) := by { left, rintro ⟨_⟩ }
-| (a :: l1) l2       :=
-  begin
-    unfold list.exteq,
-    cases (l2.remove_one a),
-    { left, rintro ⟨_⟩ },
-    apply decidable_exteq,
+    apply exists_mem_map_iff
   end
 
 end list
