src/tactic/vampire/test.lean
@@ -1,18 +1,81 @@
-
 /-
   Copyright (c) 2019 Seul Baek. All rights reserved.
   Released under Apache 2.0 license as described in the file LICENSE.
   Author: Seul Baek
 -/
 
-import tactic.vampire.main
-import tactic.vampire.main
 
-
-meta def vtest : tactic unit :=
-vampire.vampire none >> vampire
+import .main
 
 section
+
+/- Examples from finish. -/
+
+variables {A B C D : Prop}
+
+example : (A → B ∨ C) → (B → D) → (C → D) → A → D :=
+by vampire "n100ean1ean100ean10ean1n0ean11eartrrrr"
+
+example : ¬ A → A → C :=
+by vampire
+
+example : (A ∧ A ∧ B) → (A ∧ C ∧ B) → A :=
+by vampire
+
+example : A → ¬ B → ¬ (A → B) :=
+by vampire
+
+example : A ∨ B → B ∨ A :=
+by vampire
+
+example : A ∧ B → B ∧ A :=
+by vampire
+
+example : A → (A → B) → (B → C) → C :=
+by vampire
+
+example : (A ∧ B) → (C ∧ B) → C :=
+by vampire
+
+example : A → B → C → D → (A ∧ B) ∧ (C ∧ D) :=
+by vampire
+
+example : (A ∧ B) → (B ∧ ¬ C) → A ∨ C :=
+by vampire
+
+example : (A → B) ∧ (B → C) → A → C :=
+by vampire
+
+
+example : (A → B) ∨ (B → A) :=
+by vampire
+
+example : ((A → B) → A) → A :=
+by vampire
+
+example : A → ¬ B → ¬ (A → B) :=
+by vampire
+
+example : ¬ (A ↔ ¬ A) :=
+by vampire
+
+example : (A ↔ B) → (A ∧ B → C) → (¬ A ∧ ¬ B → C) → C :=
+by vampire
+
+example : (A ↔ B) → ((A ∧ ¬ B) ∨ (¬ A ∧ B)) → C :=
+by vampire
+
+example : (A → B) → A → B :=
+by vampire
+
+example : (A → B) → (B → C) → A → C :=
+by vampire
+
+example : (A → B ∨ C) → (B → D) → (C → D) → A → D :=
+by vampire
+
+example : A ∨ B → B ∨ A :=
+by vampire
 
 variables (α : Type) [inhabited α]
 variables (a b c : α) (p q : α → Prop) (r : α → α → Prop)
@@ -20,49 +83,49 @@ variables (P Q R : Prop)
 variable  (g : bool → nat)
 
 example : (∀ x, p x → q x) → (∀ x, p x) → q a :=
-by vtest
+by vampire
 
 example : (p a) → ∃ x, p x :=
-by vtest
+by vampire
 
 example : (p a) → (p b) → (q b) → ∃ x, p x ∧ q x :=
-by vtest
+by vampire
 
 example : (∃ x, p x ∧ r x x) → (∀ x, r x x → q x) → ∃ x, p x ∧ q x :=
-by vtest
+by vampire
 
 example : (∃ x, q x ∧ p x) → ∃ x, p x ∧ q x :=
-by vtest
+by vampire
 
 example : (∀ x, q x → p x) → (q a) → ∃ x, p x :=
-by vtest
+by vampire
 
 example : (∀ x, p x → q x → false) → (p a) → (p b) → (q b) → false :=
-by vtest
+by vampire
 
 example : (∀ x, p x) → (∀ x, p x → q x) → ∀ x, q x :=
-by vtest
+by vampire
 
 example : (∃ x, p x) → (∀ x, p x → q x) → ∃ x, q x :=
-by vtest
+by vampire
 
 example : (¬ ∀ x, ¬ p x) → (∀ x, p x → q x) → (∀ x, ¬ q x) → false :=
-by vtest
+by vampire
 
 example : (p a) → (p a → false) → false :=
-by vtest
+by vampire
 
 example : (¬ (P → Q ∨ R)) → (¬ (Q ∨ ¬ R)) → false :=
-by vtest
+by vampire
 
 example : (P → Q ∨ R) → (¬ Q) → P → R :=
-by vtest
+by vampire
 
 example : (∃ x, p x → P) ↔ (∀ x, p x) → P :=
-by vtest
+by vampire
 
 example : (∃ x, P → p x) ↔ (P → ∃ x, p x) :=
-by vtest
+by vampire
 
 end
 
@@ -79,31 +142,20 @@ lemma gilmore_1 {F G H : α → Prop} :
       ((F y → H y) ↔ G x) ∧
       (((F y → G y) → H y) ↔ H x)
       → F z ∧ G z ∧ H z :=
-by vtest
-
-#exit
+by vampire
 
 lemma gilmore_6 {F G : α → α → Prop} {H : α → α → α → Prop} :
 ∀ x, ∃ y,
   (∃ u, ∀ v, F u x → G v u ∧ G u x)
    → (∃ u, ∀ v, F u y → G v u ∧ G u y) ∨
        (∀ u v, ∃ w, G v u ∨ H w y u → G u w) :=
-by vtest
-"
-n101en0n11sn0spmn11n0sman0en11n0smn10n1sn0spman10en11n100smn
-1n11sn0spmarr
-"
+by vampire
 
 lemma gilmore_8 {G : α → Prop} {F : α → α → Prop} {H : α → α → α → Prop} :
   ∃ x, ∀ y z,
     ((F y z → (G y → (∀ u, ∃ v, H u v x))) → F x x) ∧
     ((F z x → G x) → (∀ u, ∃ v, H u v z)) ∧
-    F x y → F z z := by vtest
-"
-n110en10n11sn10sn0sppman10en10n10sn11sn10sn0spppmn1n0sn11sn1
-0sn0spppn1sn10sn11sn10sn0spppppman1n100en10n11sn10sn0sppmn0n
-1sn10sn11sn10sn0sppppmatrrn110en10n0sman1n1en10n10sn0spmatrr
-"
+    F x y → F z z := by vampire
 
 lemma manthe_and_bry (agatha butler charles : α)
 (lives : α → Prop) (killed hates richer : α → α → Prop) :
@@ -119,13 +171,7 @@ lemma manthe_and_bry (agatha butler charles : α)
    → killed agatha agatha ∧
        ¬ killed butler agatha ∧
        ¬ killed charles agatha :=
-by vtest
-"
-n10n1011en0n10smatn1010en1n11sman1000earrn1010en1n1sman111ea
-rrn1n101en100n1smn101n10smatn1n1001en10n10smatrn1n110en11n1s
-matn100en100n1smn101n11sman10n1n10n1100ean11eartcttcrrn111ea
-rrn1earr
-"
+by vampire
 
 /- A logic puzzle by Raymond Smullyan. -/
 
@@ -144,11 +190,97 @@ lemma knights_and_knaves (me : α) (knight knave rich poor : α → α)
     (∀ X Y Z, a_truth (and X Y) Z ∨ ¬ a_truth X Z ∨ ¬ a_truth Y Z ) ∧
     (∀ X, ¬ says me X ∨ ¬ a_truth (and (knave me) (rich me)) X ) ∧
     (∀ X, says me X ∨ a_truth (and (knave me) (rich me)) X ) ) → false :=
-by vtest
+by vampire
 
+#print knights_and_knaves
 #exit
+n10n0en11101n100sn0sn101sppn1sn101sppmn11110n101sman10n10n1n
+1011en1n100sn0sn101sppn1sn101sppmatn1010en10n100sn0sn101sppn
+1sn101sppmn11n10sn101spmn100n1sn101spmartn1n110en1110n100sn0
+sn101sppn1sn101sppmn1111n11sn101spmn10000n101sman1n1en11011n
+100sn0sn101sppn1sn101sppmn11100n101smatrn1n1n10en11001n11sn1
+01spmn11010n101smatn1n10n111en1011n11sn101spmn1100n11sn101sp
+mn1101n101sman1000en1000n11sn101spmn1010n1sn101spmn1001n10sn
+101spman1n1100en0n11sn101spmatrrtctrn1001en101n11sn101spmn11
+0n10sn101spmn111n1sn101spman1n1100en0n11sn101spmatrrtcrn1n11
+en10111n100sn0sn101sppn1sn101sppmn11000n101smatrtrtrtcn1001e
+n101n100sn0sn101sppn1sn101sppmn110n1sn101spmn111n0sn101spman
+1n10n1n1n100en10100n100sn0sn101sppn1sn101sppmn10101n100sn0sn
+101sppn1sn101sppmn10110n101sman1n10n0en11101n100sn0sn101sppn
+1sn101sppmn11110n101sman10n10n1n1011en1n100sn0sn101sppn1sn10
+1sppmatn1010en10n100sn0sn101sppn1sn101sppmn11n10sn101spmn100
+n1sn101spmartn1n110en1110n100sn0sn101sppn1sn101sppmn1111n11s
+n101spmn10000n101sman1n1en11011n100sn0sn101sppn1sn101sppmn11
+100n101smatrn1n1n10en11001n11sn101spmn11010n101smatn1n10n111
+en1011n11sn101spmn1100n11sn101spmn1101n101sman1000en1000n11s
+n101spmn1010n1sn101spmn1001n10sn101spman1n1100en0n11sn101spm
+atrrtctrn1001en101n11sn101spmn110n10sn101spmn111n1sn101spman
+1n1100en0n11sn101spmatrrtcrn1n11en10111n100sn0sn101sppn1sn10
+1sppmn11000n101smatrtrtrtcn1n1en11011n100sn0sn101sppn1sn101s
+ppmn11100n101smatrtrn10n111en1011n100sn0sn101sppn1sn101sppmn
+1100n100sn0sn101sppn1sn101sppmn1101n101sman1000en1000n100sn0
+sn101sppn1sn101sppmn1010n1sn101spmn1001n10sn101spman1n1100en
+0n100sn0sn101sppn1sn101sppmatrrtcrtn1n10n10n1n11n1n10n101en1
+0001n100sn0sn101sppn1sn101sppmn10010n100sn0sn101sppn1sn101sp
+pmn10011n101sman1n10n0en11101n100sn0sn101sppn1sn101sppmn1111
+0n101sman10n10n1n1011en1n100sn0sn101sppn1sn101sppmatn1010en1
+0n100sn0sn101sppn1sn101sppmn11n10sn101spmn100n1sn101spmartn1
+n110en1110n100sn0sn101sppn1sn101sppmn1111n11sn101spmn10000n1
+01sman1n1en11011n100sn0sn101sppn1sn101sppmn11100n101smatrn1n
+1n10en11001n11sn101spmn11010n101smatn1n10n111en1011n11sn101s
+pmn1100n11sn101spmn1101n101sman1000en1000n11sn101spmn1010n1s
+n101spmn1001n10sn101spman1n1100en0n11sn101spmatrrtctrn1001en
+101n11sn101spmn110n10sn101spmn111n1sn101spman1n1100en0n11sn1
+01spmatrrtcrn1n11en10111n100sn0sn101sppn1sn101sppmn11000n101
+smatrtrtrtcn1n1en11011n100sn0sn101sppn1sn101sppmn11100n101sm
+atrtrtn10n111en1011n100sn0sn101sppn1sn101sppmn1100n100sn0sn1
+01sppn1sn101sppmn1101n101sman1000en1000n100sn0sn101sppn1sn10
+1sppmn1010n1sn101spmn1001n10sn101spman1n1100en0n100sn0sn101s
+ppn1sn101sppmatrrtcrtn10n100en10100n100sn0sn101sppn1sn101spp
+mn10101n100sn0sn101sppn1sn101sppmn10110n101sman10n111en1011n
+100sn0sn101sppn1sn101sppmn1100n100sn0sn101sppn1sn101sppmn110
+1n101sman1n1en11011n100sn0sn101sppn1sn101sppmn11100n101smatr
+trn10n111en1011n100sn0sn101sppn1sn101sppmn1100n100sn0sn101sp
+pn1sn101sppmn1101n101sman1000en1000n100sn0sn101sppn1sn101spp
+mn1010n1sn101spmn1001n10sn101spman1n1100en0n100sn0sn101sppn1
+sn101sppmatrrtcrtrtcttctctrttctcrrn1n0en11101n1sn101spmn1111
+0n101smatn1n10n1n1n100en10100n1sn101spmn10101n1sn101spmn1011
+0n101sman1n10n0en11101n1sn101spmn11110n101sman10n10n1n1011en
+1n1sn101spmatn1010en10n1sn101spmn11n10sn101spmn100n1sn101spm
+artn1n110en1110n1sn101spmn1111n11sn101spmn10000n101sman1n1en
+11011n1sn101spmn11100n101smatrn1n1n10en11001n11sn101spmn1101
+0n101smatn1n10n111en1011n11sn101spmn1100n11sn101spmn1101n101
+sman1000en1000n11sn101spmn1010n1sn101spmn1001n10sn101spman1n
+1100en0n11sn101spmatrrtctrn1001en101n11sn101spmn110n10sn101s
+pmn111n1sn101spman1n1100en0n11sn101spmatrrtcrn1n11en10111n1s
+n101spmn11000n101smatrtrtrtcn1n1en11011n1sn101spmn11100n101s
+matrtrn10n111en1011n1sn101spmn1100n1sn101spmn1101n101sman100
+0en1000n1sn101spmn1010n1sn101spmn1001n10sn101spman1n1100en0n
+1sn101spmatrrtcrtn1n10n10n1n11n1n10n101en10001n1sn101spmn100
+10n1sn101spmn10011n101sman1n10n0en11101n1sn101spmn11110n101s
+man10n10n1n1011en1n1sn101spmatn1010en10n1sn101spmn11n10sn101
+spmn100n1sn101spmartn1n110en1110n1sn101spmn1111n11sn101spmn1
+0000n101sman1n1en11011n1sn101spmn11100n101smatrn1n1n10en1100
+1n11sn101spmn11010n101smatn1n10n111en1011n11sn101spmn1100n11
+sn101spmn1101n101sman1000en1000n11sn101spmn1010n1sn101spmn10
+01n10sn101spman1n1100en0n11sn101spmatrrtctrn1001en101n11sn10
+1spmn110n10sn101spmn111n1sn101spman1n1100en0n11sn101spmatrrt
+crn1n11en10111n1sn101spmn11000n101smatrtrtrtcn1n1en11011n1sn
+101spmn11100n101smatrtrtn10n111en1011n1sn101spmn1100n1sn101s
+pmn1101n101sman1000en1000n1sn101spmn1010n1sn101spmn1001n10sn
+101spman1n1100en0n1sn101spmatrrtcrtn10n100en10100n1sn101spmn
+10101n1sn101spmn10110n101sman10n111en1011n1sn101spmn1100n1sn
+101spmn1101n101sman1n1en11011n1sn101spmn11100n101smatrtrn10n
+111en1011n1sn101spmn1100n1sn101spmn1101n101sman1000en1000n1s
+n101spmn1010n1sn101spmn1001n10sn101spman1n1100en0n1sn101spma
+trrtcrtrtcttctctrttctcrn10n1000en1000n1sn101spmn1010n0sn101s
+pmn1001n1sn101spman1n111en1011n1sn101spmn1100n100sn0sn101spp
+n1sn101sppmn1101n101sman1n1en11011n1sn101spmn11100n101smatrt
+rtcrr
 
--- To do : find a way to avoid deep recursion with large proofs
+
+
+
 "
 n10n0en11101n110sn1sn111sppn10sn111sppmn11110n111sman10n10n1
 n1011en1n110sn1sn111sppn10sn111sppmatn1010en10n110sn1sn111sp
